construction of initial global state wip

ViperBoogieBasicRel.thy
@@ -405,6 +405,13 @@ fun boogie_const_val :: "boogie_const => ('a vbpl_val)"
   | "boogie_const_val CNull = AbsV (ARef Null)"
   | "boogie_const_val CZeroMask = AbsV (AMask zero_mask_bpl)"
 
+fun boogie_const_ty :: "'a ty_repr_bpl \<Rightarrow> boogie_const => bpl_ty"
+  where
+    "boogie_const_ty T CNoPerm = TPrim TReal"
+  | "boogie_const_ty T CWritePerm = TPrim TReal"
+  | "boogie_const_ty T CNull = TConSingle (TRefId T)"
+  | "boogie_const_ty T CZeroMask = TConSingle (TMaskId T)"
+
 definition boogie_const_rel :: "(boogie_const \<Rightarrow> vname) \<Rightarrow> var_context \<Rightarrow> ('a vbpl_absval) nstate \<Rightarrow> bool"
   where "boogie_const_rel C \<Lambda> ns \<equiv> 
            \<forall>const. lookup_var \<Lambda> ns (C const) = Some (boogie_const_val const)"
